uexp/src/uexp/cosette_tactics.lean
@@ -1,9 +1,17 @@
+import system.io
+open nat io
+open list io
+
 section cosette_tactics
 
 def list.swap_ith_forward {α : Type} {f : Type → Type} [alternative f]
-  : nat → list α → f (list α)
+    : nat → list α → f (list α)
 | 0 (x::y::zs) := pure $ y :: x :: zs
 | (nat.succ n) (x::xs) := list.cons x <$> list.swap_ith_forward n xs
 | _ _ := failure
+
+-- repeat tacitic t exactly n times
+meta def repeat_n (n: nat) (t: tactic unit) : tactic unit :=
+    nat.repeat (λ n next, t >> next) n $ return ()
 
 end cosette_tactics
